src/SMT_terms.v
@@ -811,11 +811,11 @@ Module Atom.
    | UO_Zneg
    | UO_Zopp
    | UO_BVzextn (n: nat) (i: nat)
-   | UO_BVsextn (n: nat) (i: nat).
+   | UO_BVsextn (n: nat) (i: nat)
+   | UO_BVneg   (_: nat).
 (*
    | UO_BVbitOf (_: N) (_: nat)
    | UO_BVnot   (_: N)
-   | UO_BVneg   (_: N)
    | UO_BVextr  (i: N) (n0: N) (n1: N)
 *)
 
@@ -882,10 +882,11 @@ Module Atom.
    | UO_Zopp, UO_Zopp => true
    | UO_BVzextn s1 i1, UO_BVzextn s2 i2 => Nat.eqb s1 s2 && Nat.eqb i1 i2
    | UO_BVsextn s1 i1, UO_BVsextn s2 i2 => Nat.eqb s1 s2 && Nat.eqb i1 i2
+   | UO_BVneg s1, UO_BVneg s2 => Nat.eqb s1 s2
 (*
    | UO_BVbitOf s1 n, UO_BVbitOf s2 m => Nat_eqb n m && N.eqb s1 s2
    | UO_BVnot s1, UO_BVnot s2 => N.eqb s1 s2
-   | UO_BVneg s1, UO_BVneg s2 => N.eqb s1 s2
+
    | UO_BVextr i0 n00 n01, UO_BVextr i1 n10 n11 => N.eqb i0 i1 && N.eqb n00 n10 && N.eqb n01 n11
 
 *)
@@ -960,10 +961,12 @@ Module Atom.
 
   Lemma reflect_uop_eqb : forall o1 o2, reflect (o1 = o2) (uop_eqb o1 o2).
   Proof.
-    intros [ | | | | | | ] [ | | | | | | ]; simpl; try constructor;trivial; try discriminate.
+    intros [ | | | | | | | ] [ | | | | | | | ]; simpl; try constructor;trivial; try discriminate.
     intros. preflect (Nat.eqb_spec n n0). preflect (Nat.eqb_spec i i0).  rewrite Heq, Heq0.
     now constructor.
     intros. preflect (Nat.eqb_spec n n0). preflect (Nat.eqb_spec i i0).  rewrite Heq, Heq0.
+    now constructor.
+    intros. preflect (Nat.eqb_spec n n0). rewrite Heq.
     now constructor.
   Qed.
 
@@ -1174,10 +1177,11 @@ Qed.
         | UO_Zopp => (Typ.TZ, Typ.TZ)
         | UO_BVzextn s i => (Typ.TWord s, Typ.TWord (i + s))
         | UO_BVsextn s i => (Typ.TWord s, Typ.TWord (i + s))
+        | UO_BVneg s => (Typ.TWord s, Typ.TWord s)
 (*
         | UO_BVbitOf s _ => (Typ.TBV s, Typ.Tbool)
         | UO_BVnot s => (Typ.TBV s, Typ.TBV s)
-        | UO_BVneg s => (Typ.TBV s, Typ.TBV s)
+
         | UO_BVextr i n0 n1 => (Typ.TBV n1, Typ.TBV n0)
 
 *)
@@ -1593,10 +1597,11 @@ Qed.
           apply_unop (Typ.TWord s) (Typ.TWord (s + i)) (fun w => @zext s w i)
         | UO_BVsextn s i => 
           apply_unop (Typ.TWord s) (Typ.TWord (s + i)) (fun w => @sext s w i)
+        | UO_BVneg s => apply_unop (Typ.TWord s) (Typ.TWord s) (@wneg s)
 (*
         | UO_BVbitOf s n => apply_unop (Typ.TBV s) Typ.Tbool (BITVECTOR_LIST.bitOf n)
         | UO_BVnot s => apply_unop (Typ.TBV s) (Typ.TBV s) (@BITVECTOR_LIST.bv_not s)
-        | UO_BVneg s => apply_unop (Typ.TBV s) (Typ.TBV s) (@BITVECTOR_LIST.bv_neg s)
+
         | UO_BVextr i n0 n1 => 
           apply_unop (Typ.TBV n1) (Typ.TBV n0) (@BITVECTOR_LIST.bv_extr i n0 n1)
 *)
@@ -2140,17 +2145,19 @@ Qed.
             destruct H as [ H | H].
               rewrite Nat.eqb_refl in H. now contradict H.
               now rewrite H.
+            (* bv_neg *)
+            specialize (H (Typ.TWord n)). simpl in H. rewrite andb_false_iff in H.
+            destruct H as [ H | H].
+              rewrite Nat.eqb_refl in H. now contradict H.
+              now rewrite H.
+
 (*
             (* bv_not *)
             specialize (H (Typ.TBV n)). simpl in H. rewrite andb_false_iff in H.
             destruct H as [ H | H].
               rewrite N.eqb_refl in H. now contradict H.
               now rewrite H.
-            (* bv_neg *)
-            specialize (H (Typ.TBV n)). simpl in H. rewrite andb_false_iff in H.
-            destruct H as [ H | H].
-              rewrite N.eqb_refl in H. now contradict H.
-              now rewrite H.
+
             (* bv_extr *)
             specialize (H (Typ.TBV n0)). simpl in H. rewrite andb_false_iff in H.
             destruct H as [ H | H].
